examples/counter/extraction/CameLIGOCounter.v
@@ -10,6 +10,7 @@ From ConCert.Extraction Require Import Common.
 From ConCert.Extraction Require Import CameLIGOPretty.
 From ConCert.Extraction Require Import CameLIGOExtract.
 From ConCert.Execution Require Import Blockchain.
+From ConCert.Execution Require Import ResultMonad.
 
 Import MCMonadNotation.
 
@@ -29,7 +30,8 @@ Module Counter.
   Definition operation := ActionBody.
   Definition storage := Z × address.
 
-  Definition init (setup : Z * address) : option storage := Some setup.
+  Definition init (setup : Z * address) : result storage unit :=
+    Ok setup.
 
   Inductive msg :=
   | Inc (_ : Z)
@@ -41,17 +43,18 @@ Module Counter.
   Definition dec_balance (st : storage) (new_balance : Z) :=
     (st.1 - new_balance, st.2).
 
-  Definition counter_inner (msg : msg) (st : storage)
-    : option (list operation * storage) :=
+  Definition counter_inner (msg : msg)
+                           (st : storage)
+                           : result (list operation * storage) unit :=
     match msg with
     | Inc i =>
       if (0 <=? i) then
-        Some ([],inc_balance st i)
-      else None
+        Ok ([],inc_balance st i)
+      else Err tt
     | Dec i =>
       if (0 <=? i) then
-        Some ([],dec_balance st i)
-      else None
+        Ok ([],dec_balance st i)
+      else Err tt
     end.
 
   Definition counter (c : Chain) (ctx : ContractCallContext) st msg :=
@@ -60,11 +63,11 @@ Module Counter.
     let c_ := c in
     let ctx_ := ctx in
     match msg with
-    | Some msg =>counter_inner msg st
-    | None => None
+    | Some msg => counter_inner msg st
+    | None => Err tt
     end.
 
-  Definition LIGO_COUNTER_MODULE : CameLIGOMod msg _ (Z × address) storage operation :=
+  Definition LIGO_COUNTER_MODULE : CameLIGOMod msg _ (Z × address) storage operation unit :=
     {| (* a name for the definition with the extracted code *)
         lmd_module_name := "cameLIGO_counter" ;
 
